remove copy from rot32bits

Clean/Gadgets/Rotation32/Rotation32.lean
@@ -37,8 +37,8 @@ def spec (offset : Fin 32) (x : U32 (F p)) (y: U32 (F p)) :=
 -- #eval! (rot32 (p:=p_babybear) 0) default |>.output
 def elaborated (off : Fin 32) : ElaboratedCircuit (F p) U32 U32 where
   main := rot32 off
-  local_length _ := 12
-  output _inputs i0 := var_from_offset U32 (i0 + 8)
+  local_length _ := 8
+  output _inputs i0 := Rotation32Bits.output (off % 8).val i0
 
 theorem soundness (offset : Fin 32) : Soundness (F p) (circuit := elaborated offset) assumptions (spec offset) := by
   intro i0 env x_var x h_input x_normalized h_holds
@@ -56,7 +56,7 @@ theorem soundness (offset : Fin 32) : Soundness (F p) (circuit := elaborated off
     Vector.finRange] at h_holds
 
   simp [circuit_norm, spec, h_holds, elaborated]
-  set y := eval env (var_from_offset U32 (i0 + 8))
+  set y := eval env (Rotation32Bits.output (offset.val % 8 : ℕ) i0)
 
   simp [assumptions] at x_normalized
   rw [←h_input] at x_normalized
